Existential HL linking proofs.

theories/Imp.v
@@ -23,7 +23,8 @@ Ltac split_and :=
 Require Import
         Coq.Bool.Bool
         Coq.Strings.String
-        Coq.Lists.List.
+        Coq.Lists.List
+        Coq.Sets.Ensembles.
 
 Import Nat.
 Require Import Maps.
@@ -194,7 +195,7 @@ Inductive ceval (Sigma : Env) : com -> state -> state -> Type :=
       (funSpecs f).(post) n (aseval st args) ->
       Sigma |- st =[ x :::= f $ args ]=> (x !-> n ; st)
 
-  | E_CallImpl : forall st st' args fd x f,
+  | E_CallDef : forall st st' args fd x f,
       funDefs f = Some fd ->
       Sigma |- build_total_map (funArgs fd) (aseval st args) 0 =[ funBody fd ]=> st' ->
       Sigma |- st =[ x :::= f $ args ]=> (x !-> aeval st' (funRet fd); st)
@@ -343,7 +344,7 @@ Section safe_Execution.
     - econstructor; eauto; simpl in *.
       unfold update, t_update; find_if_inside; subst; eauto.
       destruct H; eauto.
-    - eapply E_CallImpl; simpl; eauto.
+    - eapply E_CallDef; simpl; eauto.
       unfold update, t_update; find_if_inside; eauto.
       destruct H; subst; eauto.
   Qed.
@@ -369,7 +370,7 @@ Section safe_Execution.
     - econstructor; eauto; simpl in *.
       unfold update, t_update in *; find_if_inside; subst; eauto;
         discriminate.
-    - eapply E_CallImpl; simpl in *; eauto.
+    - eapply E_CallDef; simpl in *; eauto.
       + eapply update_inv in e; destruct e as [[? ?] | [? ?]];
           subst; eauto.
         destruct H; eauto.
@@ -562,6 +563,93 @@ Section productive_Execution.
      this should feel free to suggest another. Living? NotDead? UnDead?
      *)
 
+  (* A productive initial state is one that ensures the program
+  *always* produces the specified final state *)
+
+  Local Arguments Singleton [_] _.
+
+  Inductive Productive (Sigma : Env) : com -> state -> Ensemble state -> Prop :=
+    | Productive_Skip : forall st,
+        Productive Sigma SKIP st (Singleton st)
+    | Productive_Ass  : forall st x a,
+        Productive Sigma (x ::= a) st (Singleton (x !-> (aeval st a) ; st))
+    | Productive_Seq : forall c1 c2 st Q Q',
+        Productive Sigma c1 st Q ->
+        (forall st', Q st' -> Productive Sigma c2 st' Q') ->
+         Productive Sigma (c1 ;; c2) st Q'
+    | Productive_IfTrue : forall st Q b c1 c2,
+        beval st b = true ->
+        Productive Sigma c1 st Q ->
+        Productive Sigma (TEST b THEN c1 ELSE c2 FI) st Q
+    | Productive_IfFalse : forall st b c1 c2 Q,
+        beval st b = false ->
+        Productive Sigma c2 st Q ->
+        Productive Sigma (TEST b THEN c1 ELSE c2 FI) st Q
+    | Productive_WhileFalse : forall b st c,
+        beval st b = false ->
+        Productive Sigma (WHILE b DO c END) st (Singleton st)
+    | Productive_WhileTrue : forall st b c Q Q',
+        beval st b = true ->
+        Productive Sigma c st Q ->
+        (forall st', Q st' ->
+                     Productive Sigma (WHILE b DO c END) st' Q') ->
+        Productive Sigma (WHILE b DO c END) st Q'
+    | Productive_CallDef :
+        forall st Q args x f fd,
+          funDefs f = Some fd ->
+          Productive Sigma (funBody fd) (build_total_map (funArgs fd) (aseval st args) 0) Q
+          -> Productive Sigma (x :::= f $ args) st
+                        (fun st' => exists st'', Q st'' /\ st' = (x !-> aeval st'' (funRet fd); st))
+    | Productive_CallSpec : forall st args x f n,
+        funDefs f = None ->
+        (funSpecs f).(pre) (aseval st args) ->
+        (funSpecs f).(post) n (aseval st args) ->
+        Productive Sigma (x :::= f $ args) st
+                   (fun st' => exists n, (funSpecs f).(post) n (aseval st args)
+                                         /\ st' = (x !-> n; st))
+    | Productive_Weaken : forall st c Q Q',
+        Productive Sigma c st Q ->
+        Included state Q Q' ->
+        Productive Sigma c st Q'.
+
+  (* Productivity is a *stronger* property than evaluation-- it forces
+     a command to evaluate to a final state regardless of how
+     nondeterministic choices are made. *)
+  Theorem productive_com_produces (Sigma : Env) :
+    forall (c : com) (st : state) (Q : Ensemble state),
+      Productive Sigma c st Q ->
+      exists st' (exe : Sigma |- st =[c]=> st'), Q st'.
+  Proof.
+    induction 1.
+    - assert (Sigma |- st =[ SKIP ]=> st) by econstructor.
+      eexists _, X; econstructor.
+    - eassert (Sigma |- st =[ x ::= a ]=> _) by (econstructor; eauto).
+      eexists _, X; econstructor.
+    - destruct IHProductive as [st' [exe Q_st'] ].
+      specialize (H0 _ Q_st'); destruct (H1 _ Q_st') as [st'' [exe' Q'_st']].
+      assert (Sigma |- st =[ c1;; c2 ]=> st'') by (econstructor; eauto).
+      eauto.
+    - destruct IHProductive as [st' [exe Q_st'] ].
+      assert (Sigma |- st =[ TEST b THEN c1 ELSE c2 FI ]=> st') by (econstructor; eauto).
+      eexists _, X ; eauto.
+    - destruct IHProductive as [st' [exe Q_st'] ].
+      assert (Sigma |- st =[ TEST b THEN c1 ELSE c2 FI ]=> st') by (econstructor; eauto).
+      eexists _, X; eauto.
+    - assert (Sigma |- st =[ WHILE b DO c END ]=> st) by (econstructor; eauto).
+      eexists _, X; eauto; econstructor.
+    - destruct IHProductive as [st' [exe Q_st'] ].
+      specialize (H1 _ Q_st'); destruct (H2 _ Q_st') as [st'' [exe' Q'_st']].
+      assert (Sigma |- st =[ WHILE b DO c END ]=> st'') by (econstructor; eauto).
+      eauto.
+    - destruct IHProductive as [st' [exe Q_st'] ].
+      eassert (Sigma |- st =[ x :::= f $ args ]=> _) by (eapply (@E_CallDef Sigma); eauto).
+      eexists _, X; eauto.
+    - eassert (Sigma |- st =[ x :::= f $ args ]=> _) by (eapply (@E_CallSpec Sigma); eauto).
+      eexists _, X; eauto.
+    - destruct IHProductive as [st' [exe Q_st'] ]; eexists _, exe; eauto.
+      eapply H0; apply Q_st'.
+  Qed.
+
   (* A productive function definition is one that produces at least
      one behavior allowed by its specifiction. *)
   Definition productive_funDef (Sigma : Env)
@@ -569,9 +657,8 @@ Section productive_Execution.
              (fd : funDef) : Prop :=
     forall (args : list nat),
       (pre fs) args ->
-      exists (st' : state)
-             (exe : Sigma |- build_total_map (funArgs fd) args 0 =[ funBody fd ]=> st'),
-        (post fs) (aeval st' (funRet fd)) args.
+      exists Q (exe : Productive Sigma (funBody fd) (build_total_map (funArgs fd) args 0) Q),
+        forall st', Q st' -> (post fs) (aeval st' (funRet fd)) args.
 
   (* An environment is productive if all of its function definitions are
      productive with respect to their specs.  *)
@@ -580,89 +667,35 @@ Section productive_Execution.
       funDefs f = Some fd ->
       productive_funDef Sigma (funSpecs f) fd.
 
-  (* A productive initial state is one that ensures the program
-  *always* produces the specified final state *)
+  Lemma productive_empty
+    : forall Sigs Sigma,
+      productive_Env {| funSigs := Sigs; funSpecs := Sigma; funDefs := empty |}.
+    unfold productive_Env; simpl; intros; discriminate.
+  Qed.
 
-  (*CoInductive Productive (Sigma : Env) : com -> state -> state -> Type :=
-    | Productive_Skip : forall st,
-        Productive Sigma SKIP st st
-    | Productive_Ass  : forall st x a,
-        Productive Sigma (x ::= a) st (x !-> (aeval st a) ; st)
-    | Productive_Seq : forall c1 c2 st st'',
-        (forall st', Sigma |- st =[ c1 ]=> st' -> Productive Sigma c2 st' st'') ->
-        Productive Sigma (c1 ;; c2) st st''
-    | Productive_IfTrue : forall st st' b c1 c2,
-        beval st b = true ->
-        Productive Sigma c1 st st' ->
-        Productive Sigma (TEST b THEN c1 ELSE c2 FI) st st'
-    | Productive_IfFalse : forall st b c1 c2 st',
-        beval st b = false ->
-        Productive Sigma c2 st st' ->
-        Productive Sigma (TEST b THEN c1 ELSE c2 FI) st st'
-    | Productive_WhileFalse : forall b st c,
-        beval st b = false ->
-        Productive Sigma (WHILE b DO c END) st st
-    | Productive_WhileTrue : forall st b c st'',
-        beval st b = true ->
-        (forall st', Sigma |- st =[ c ]=> st' ->
-                     Productive Sigma (WHILE b DO c END) st' st'') ->
-        Productive Sigma (WHILE b DO c END) st st''
-    | Productive_CallDef :
-        forall st st' args x f fd,
-          funDefs f = Some fd ->
-          Productive Sigma (funBody fd) (build_total_map (funArgs fd) (aseval st args) 0) st'
-          -> Productive Sigma (x :::= f $ args) st (x !-> aeval st' (funRet fd); st)
-    | Productive_CallSpec : forall st args x f n,
-        funDefs f = None ->
-        (funSpecs f).(pre) (aseval st args) ->
-        (funSpecs f).(post) n (aseval st args) ->
-        Productive Sigma (x :::= f $ args) st (x !-> n ; st). *)
-
-  (* Key Productivity Theorem: executing a program in a productive
+    (* Key Productivity Theorem: executing a program in a productive
   environment and productive initial state will produce some value that a
   'pure' specification environment (i.e. one without any function
   definitions) would have. *)
-
-  (*Theorem productive_Env_produces (Sigma : Env) :
-    forall (c : com) (st st' : state),
+  Theorem productive_Env_produces (Sigma : Env) :
+    forall (c : com) (st : state) (Q : Ensemble state),
       productive_Env Sigma ->
       Productive {|
           funSigs := funSigs;
           funSpecs := funSpecs;
-          funDefs := empty |} c st ->
-      { st'' : state & ((Sigma |- st =[ c ]=> st'') *
-      ({| funSigs := funSigs;
-          funSpecs := funSpecs;
-          funDefs := empty |} |- st =[ c ]=> st''))%type}.
+          funDefs := empty |} c st Q ->
+      Productive Sigma c st Q.
   Proof.
-    induction c; intros st Prod_Sig Safe_Sig;
-      try (solve [eexists _; split; econstructor; eauto]).
-    - admit.
-    - inversion Safe_Sig; subst; clear Safe_Sig.
-      destruct (IHc1 _ Prod_Sig X) as [st' [? ?] ].
-      specialize (X0 _ c0).
-      destruct (IHc2 _ Prod_Sig X0) as [st'' [? ?] ].
-      exists st''; split; econstructor; eauto.
-    - inversion Safe_Sig; subst; clear Safe_Sig.
-      + destruct (IHc1 _ Prod_Sig X) as [st' [? ?] ].
-        exists st'; split; econstructor; eauto.
-      + destruct (IHc2 _ Prod_Sig X) as [st' [? ?] ].
-        exists st'; split; eapply E_IfFalse; eauto.
-    - inversion Safe_Sig; subst; clear Safe_Sig.
-      + exists st; split; econstructor; eauto.
-      + destruct (IHc _ Prod_Sig X) as [st' [? ?] ].
-        eapply X0 in c1.
-        destruct (IHc _ Prod_Sig c1) as [st' [? ?] ].
-
-      inversion X; subst; try congruence; econstructor; eauto.
-    - inversion X; subst; try congruence; econstructor; eauto.
-    - inversion X; subst; eapply E_IfFalse; eauto; congruence.
-    - inversion X; subst; try congruence; econstructor; eauto.
-    - inversion X; subst; try congruence.
-      + simpl in *; rewrite apply_empty in H4; discriminate.
-      + eapply (E_CallSpec {| funSpecs := @funSpecs Sigma; funDefs := empty |});
-          simpl in *; eauto.
-        eapply H; eauto.
-  Qed. *)
+    induction 2; intros; try (solve [econstructor; eauto]).
+    - simpl in *; rewrite apply_empty in H0; discriminate.
+    - destruct (@funDefs Sigma f) eqn: ?.
+      + destruct (H _ _ Heqo _ H1) as [Q [exe Q_exe] ].
+        eapply Productive_Weaken.
+        econstructor; eauto.
+        unfold Included, In; intros.
+        destruct H3 as [? [? ?] ].
+        eexists (aeval x1 (funRet f0)); split; eauto.
+      + eapply (@Productive_CallSpec Sigma); eauto.
+  Qed.
 
 End productive_Execution.
